feat(*) initial support for IFs in non-final positions

HOL_To_IMP_Minus/HOL_Nat_To_IMP_Minus/Compile_HOL_Nat_To_IMP/Compile_HOL_Nat_To_IMP.thy
@@ -36,19 +36,19 @@ proof(induction c arbitrary: s t s' rule: assoc_right_tSeq.induct)
     using tIfFalse by fastforce
 qed(auto simp: tbig_step_t_tSeq_assoc intro!: Suc_eq_plus1)
 
-fun tseq where
-  "tseq tSKIP c = c"
-| "tseq c tSKIP = c"
-| "tseq c1 c2 = tSeq c1 c2"
+fun rm_tSkip_tseq where
+  "rm_tSkip_tseq tSKIP c = c"
+| "rm_tSkip_tseq c tSKIP = c"
+| "rm_tSkip_tseq c1 c2 = tSeq c1 c2"
 
 fun rm_tSKIP where
-  "rm_tSKIP (tSeq c1 c2) = tseq (rm_tSKIP c1) (rm_tSKIP c2)"
+  "rm_tSKIP (tSeq c1 c2) = rm_tSkip_tseq (rm_tSKIP c1) (rm_tSKIP c2)"
 | "rm_tSKIP (tIf v c1 c2) = tIf v (rm_tSKIP c1) (rm_tSKIP c2)"
 | "rm_tSKIP c = c"
 
-lemma tbig_step_t_tseq:
+lemma tbig_step_t_rm_tSkip_tseq:
   assumes "C \<turnstile> (c1, s0) \<Rightarrow>\<^bsup>t1\<^esup> s1" "C \<turnstile> (c2, s1) \<Rightarrow>\<^bsup>t2\<^esup> s2"
-  shows "\<exists>t'. C \<turnstile> (tseq c1 c2, s0) \<Rightarrow>\<^bsup>t'\<^esup> s2 \<and> t' \<le> t1 + t2"
+  shows "\<exists>t'. C \<turnstile> (rm_tSkip_tseq c1 c2, s0) \<Rightarrow>\<^bsup>t'\<^esup> s2 \<and> t' \<le> t1 + t2"
 proof -
   consider
     "c1 = tSKIP" | "c1 \<noteq> tSKIP" "c2 = tSKIP" | "c1 \<noteq> tSKIP" "c2 \<noteq> tSKIP"
@@ -64,7 +64,7 @@ proof -
       using tSkip by (cases c1) auto
   next
     case 3
-    then have "tseq c1 c2 = tSeq c1 c2"
+    then have "rm_tSkip_tseq c1 c2 = tSeq c1 c2"
       by (cases c1; cases c2) simp_all
     with assms show ?thesis
       using tSeq by auto
@@ -81,7 +81,7 @@ proof(induction c arbitrary: s t s' rule: rm_tSKIP.induct)
     "C \<turnstile> (rm_tSKIP c1, s) \<Rightarrow>\<^bsup>t1\<^esup> s1" "C \<turnstile> (rm_tSKIP c2, s1) \<Rightarrow>\<^bsup>t2\<^esup> s'"
     "t1 + t2 \<le> t"
     by (metis add_mono tSeq_tE)
-  with 1 show ?case using tbig_step_t_tseq by fastforce
+  with 1 show ?case using tbig_step_t_rm_tSkip_tseq by fastforce
 next
   case (2 v c1 c2)
   then show ?case
@@ -101,6 +101,16 @@ next
       unfolding rm_tSKIP.simps by force
   qed
 qed auto
+
+(*input: right-associated program*)
+(*output: all ifs are pulled out + right-associated*)
+fun pull_tIf where
+  "pull_tIf (tSeq (tIf v c1 c2) c3) = tIf v (pull_tIf (tSeq c1 c3)) (pull_tIf (tSeq c2 c3))"
+  (* "pull_tIf (tSeq (tIf v c1 c2) c3) =
+    tIf v (pull_tIf (tSeq c1 c3)) (pull_tIf (tSeq c2 c3))" *)
+| "pull_tIf (tSeq c1 c2) = tSeq c1 (pull_tIf c2)"
+| "pull_tIf (tIf v c1 c2) = tIf v (pull_tIf c1) (pull_tIf c2)"
+| "pull_tIf c = c"
 
 ML_file\<open>compile_hol_nat_to_imp.ML\<close>
 
